theories/base.v
@@ -32,3 +32,93 @@ Definition list_find_idx {A} P `{∀ x, Decision (P x)} : list A → option nat 
   | x :: l => if decide (P x) then Some 0%nat else S <$> go l
   end.
 Instance: Params (@list_find_idx) 3 := {}.
+
+Section list_find_idx.
+  Context {A} (P : A → Prop) `{∀ x, Decision (P x)}.
+
+  Lemma list_find_idx_list_find l:
+    list_find_idx P l = fst <$> list_find P l.
+  Proof.
+    elim: l => //= ?? ->. case_decide => //=.
+    rewrite -!option_fmap_compose. by apply: option_fmap_ext.
+  Qed.
+
+  Lemma list_find_idx_Some l i:
+    list_find_idx P l = Some i ↔
+    ∃ x, l !! i = Some x ∧ P x ∧ ∀ j y, l !! j = Some y → (j < i)%nat → ¬P y.
+  Proof.
+    rewrite list_find_idx_list_find fmap_Some.
+    split.
+    - move => -[[??]]. rewrite list_find_Some. naive_solver.
+    - move => [??]. eexists (_, _). rewrite list_find_Some. naive_solver.
+  Qed.
+
+  Lemma list_find_idx_lt l i:
+    list_find_idx P l = Some i → (i < length l)%nat.
+  Proof. move => /list_find_idx_Some[?[??]]. by apply: lookup_lt_Some. Qed.
+
+  Lemma list_find_idx_insert_eq l i x:
+    list_find_idx P l = Some i →
+    P x →
+    list_find_idx P (<[i:=x]> l) = Some i.
+  Proof.
+    rewrite !list_find_idx_Some => -[?[?[??]]] ?. eexists _.
+    rewrite list_lookup_insert. 2: by apply: lookup_lt_Some. split_and! => //.
+    move => ?? /list_lookup_insert_Some. naive_solver.
+  Qed.
+
+  Lemma list_find_idx_insert_neq l i j x y:
+    list_find_idx P l = Some i →
+    ¬ P x →
+    l !! j = Some y →
+    ¬ P y →
+    list_find_idx P (<[j:=x]> l) = Some i.
+  Proof.
+    rewrite !list_find_idx_Some => -[?[?[??]]] ???. eexists _.
+    rewrite list_lookup_insert_ne. 2: move => ?; by simplify_eq.
+    split_and! => //. move => ?? /list_lookup_insert_Some. naive_solver.
+  Qed.
+End list_find_idx.
+
+Section map_Forall.
+  Context `{FinMap K M}.
+  Context {A} (P : K → A → Prop).
+  Implicit Types m : M A.
+
+  Lemma map_Forall_impl' (Q : K → A → Prop) m :
+    map_Forall P m → (∀ i x, m !! i = Some x → P i x → Q i x) → map_Forall Q m.
+  Proof. unfold map_Forall; naive_solver. Qed.
+  Lemma map_Forall_insert_2' m i x :
+    P i x → map_Forall (λ j y, i ≠ j → P j y) m → map_Forall P (<[i:=x]>m).
+  Proof using Type*. intros ?? j y; rewrite lookup_insert_Some; naive_solver. Qed.
+
+End map_Forall.
+
+From iris.bi Require Import bi.
+
+Section big_op.
+Context {PROP : bi}.
+Implicit Types P Q : PROP.
+Implicit Types Ps Qs : list PROP.
+Implicit Types A : Type.
+Section sep_map.
+  Context `{Countable K} {A : Type}.
+  Implicit Types m : gmap K A.
+  Implicit Types Φ Ψ : K → A → PROP.
+  Lemma big_sepM_kmap {B} `{Countable B} (f : K → B) (Φ : B → A → PROP) m `{!Inj eq eq f}:
+    ([∗ map] k↦y ∈ kmap f m, Φ k y) ⊣⊢ ([∗ map] k↦y ∈ m, Φ (f k) y).
+  Proof.
+    induction m as [|???? IH] using map_ind => /=. { by rewrite kmap_empty !big_sepM_empty. }
+    rewrite kmap_insert !big_sepM_insert // ?IH // lookup_kmap_None => ??. by simplify_eq.
+  Qed.
+
+  Lemma big_sepM_list_to_map (Φ : K → A → PROP) l:
+    NoDup l.*1 →
+    ([∗ map] k↦y ∈ list_to_map l, Φ k y) ⊣⊢ ([∗ list] y ∈ l, Φ y.1 y.2).
+  Proof.
+    induction l as [|?? IH]; csimpl. { by rewrite !big_sepM_empty. }
+    move => /NoDup_cons[??]. rewrite big_sepM_insert ?IH //.
+    by apply: not_elem_of_list_to_map_1.
+  Qed.
+End sep_map.
+End big_op.
